@prefix : <http://www.semanticweb.org/matt.weber/ontologies/2018/10/untitled-ontology-15#> .
@prefix owl: <http://www.w3.org/2002/07/owl#> .
@prefix rdf: <http://www.w3.org/1999/02/22-rdf-syntax-ns#> .
@prefix xml: <http://www.w3.org/XML/1998/namespace> .
@prefix xsd: <http://www.w3.org/2001/XMLSchema#> .
@prefix rdfs: <http://www.w3.org/2000/01/rdf-schema#> .
@base <http://www.ptolemy.berkeley.edu/SemanticSensor> .

<http://www.ptolemy.berkeley.edu/SemanticSensor> rdf:type owl:Ontology .

#################################################################
#    Object Properties
#################################################################

###  http://www.ptolemy.berkeley.edu/SemanticSensor#Collects
:Collects rdf:type owl:ObjectProperty ;
          rdfs:domain :SemanticSensor ;
          rdfs:range :SemanticObservation .


#################################################################
#    Data properties
#################################################################

###  http://www.ptolemy.berkeley.edu/SemanticSensor#CollectionTime
:CollectionTime rdf:type owl:DatatypeProperty ;
                rdfs:domain :SemanticObservation ;
                rdfs:range xsd:dateTime ;
                rdfs:comment "The time this observation is collected and prepared for insertion to a semantic repository." .


###  http://www.ptolemy.berkeley.edu/SemanticSensor#Expires
:Expires rdf:type owl:DatatypeProperty ;
         rdfs:domain :SemanticObservation ;
         rdfs:range xsd:dateTime ;
         rdfs:comment "The timestamp at which this observation should be considered invalid and removed from the semantic repository." .


###  http://www.ptolemy.berkeley.edu/SemanticSensor#ObservationTime
:ObservationTime rdf:type owl:DatatypeProperty ;
                 rdfs:domain :SemanticObservation ;
                 rdfs:range xsd:dateTime ;
                 rdfs:comment "The time the phenomenon being recorded by this observation occurred." .


#################################################################
#    Classes
#################################################################

###  http://www.ptolemy.berkeley.edu/SemanticSensor#SemanticObservation
:SemanticObservation rdf:type owl:Class .


###  http://www.ptolemy.berkeley.edu/SemanticSensor#SemanticSensor
:SemanticSensor rdf:type owl:Class .


###  Generated by the OWL API (version 4.2.8.20170104-2310) https://github.com/owlcs/owlapi
